

## Chapter 03 Likelihood-Based Tests and Confidence Regions

### Part 02

#### 3.1 Simple Null Hypothesis

$H_0: \theta = \theta_0 \quad H_a: \theta \neq \theta_0$  where  $\theta_{b \times 1}$  and  
 $Y_1, \dots, Y_n$  are iid from  $f(y; \theta)$

The identity matrix is denoted by  $\mathbb{I}$  in the following.

The asymptotic distribution results for the three statistics stated below hold under suitable regularity conditions.

• The Wald statistic is

$$T_w = \underbrace{(\hat{\theta}_{MLE} - \theta_0)^T}_{1 \times b} \underbrace{\{I_T(\hat{\theta}_{MLE})\}}_{b \times b} \underbrace{(\hat{\theta}_{MLE} - \theta_0)}_{b \times 1}$$

$\hat{\theta}_{MLE}$  is  $AN(\theta, \{I_T(\theta)\}^{-1})$  or equivalently,

$\{I_T(\theta)\}^{-\frac{1}{2}}(\hat{\theta}_{MLE} - \theta) \xrightarrow{d} N(0, \mathbb{I}_b)$  where  $\mathbb{I}_b$  is the  $b$ -dimensional identity matrix. It follows that  $T_w \xrightarrow{d} \chi_b^2$  as  $n \rightarrow \infty$  under  $H_0$  provided  $I_T(\hat{\theta}_{MLE}) \{I_T(\theta_0)\}^{-1}$  converges in probability to  $\mathbb{I}_b$  as  $n \rightarrow \infty$  under  $H_0$ .

In fact,  $I_T(\hat{\theta}_{MLE})$  can be replaced by  $I_T(\theta_0)$  or by the sample information matrix  $I_T(Y, \hat{\theta}_{MLE})$  in the definition of  $T_w$  and the asymptotic distribution of the resulting statistic is unchanged.

• The score test statistic is

$$T_s = S(\theta_0)^T \{I_T(\theta_0)\}^{-1} S(\theta_0)$$

Under  $H_0$ ,  $S(\theta_0)$  has mean 0, variance  $I_T(\theta_0)$ , and by The Central Limit Theorem is  $AN(0, I_T(\theta_0))$ . Thus  $\{I_T(\theta_0)\}^{-\frac{1}{2}} S(\theta_0)$  converges in distribution to  $N(0, I_b)$  under  $H_0$ . It follows that  $T_s \xrightarrow{d} \chi_b^2$  as  $n \rightarrow \infty$  under  $H_0$ .

• The likelihood ratio statistic is

$$T_{LR} = -2 \log \left\{ \frac{\sup_{\theta \in H_0} L(\theta|Y)}{\sup_{\theta \in \Theta} L(\theta|Y)} \right\} = -2 \{L(\theta_0) - L(\hat{\theta}_{MLE})\}$$

where  $\Theta$  is the parameter space and  $\sup = \text{least upper bound}$  plays the role of "maximum" in cases where the maximum is not attained.

Example 3.1 (Normal model with known variance).

Suppose that  $Y_1, \dots, Y_n$  are iid  $N(\mu, 1)$  and  $H_0: \mu = \mu_0$ . Then

$$f(y) = \frac{1}{\sqrt{2\pi}} e^{-\frac{1}{2}(y-\mu)^2}$$

$$L(\mu) = (2\pi)^{-\frac{n}{2}} e^{-\frac{1}{2} \sum_{i=1}^n (Y_i - \mu)^2}$$

$$= (2\pi)^{-\frac{n}{2}} e^{-\frac{1}{2} \sum_{i=1}^n (Y_i - \mu)^2}$$

$$\ell(\mu) = \log L(\mu|Y) = -\frac{n}{2} \log(2\pi) - \frac{1}{2} \sum_{i=1}^n (Y_i - \mu)^2$$

$$S(\mu) = -\frac{1}{2} \sum_{i=1}^n (Y_i - \mu) (-2) = \sum_{i=1}^n (Y_i - \mu) \Rightarrow \hat{\mu}_{MLE} = \bar{Y}$$

$$\text{and } I_T(Y, \mu) = -\frac{\partial}{\partial \mu} S(\mu) = n,$$

so that  $\hat{\mu}_{MLE} = \bar{Y}$  and  $I_T(\mu) = E\{I_T(Y, \mu)\} = n$ .

It follows that

$$T_W = (\bar{Y} - \mu_0)(n)(\bar{Y} - \mu_0) = n(\bar{Y} - \mu_0)^2 \text{ and}$$

$$T_S = \sum_{i=1}^n (Y_i - \mu_0) (n^{-1}) \sum_{i=1}^n (Y_i - \mu_0) = \frac{1}{n} \sum_{i=1}^n (Y_i - \mu_0) \cdot \frac{1}{n} \sum_{i=1}^n (Y_i - \mu_0) n$$

$= n(\bar{Y} - \mu_0)^2$ , are identical for this model.

Example 3.2 (Bernoulli data).

Suppose that  $Y_1, \dots, Y_n$  are iid from a Bernoulli distribution with parameter  $p$  and  $H_0: p = p_0$ . With  $X = \sum_{i=1}^n Y_i$ ,

$$f(y) = p^y (1-p)^{1-y}$$

$$L(p) = \prod_{i=1}^n f(y_i) = p^{\sum y_i} (1-p)^{n - \sum y_i} = p^x (1-p)^{n-x}$$

$$l(p) = x \log p + (n-x) \log(1-p)$$

$$S(p) = \frac{\partial l(p)}{\partial p} = \frac{x}{p} - \frac{n-x}{1-p} = \frac{x(1-p)}{p(1-p)} - \frac{p(n-x)}{p(1-p)} = \frac{x - xp - pn + xp}{p(1-p)}$$

$$= \frac{x - pn}{p(1-p)} \Rightarrow \hat{p}_{MLE} = \hat{p} = \frac{x}{n}$$

$$\text{and } I_T(Y, p) = -\frac{\partial}{\partial p} S(p) = -\left(-\frac{x}{p^2} - \frac{n-x}{(1-p)^2}\right) = \frac{x}{p^2} + \frac{n-x}{(1-p)^2}$$

$$\text{Thus } \hat{p}_{MLE} = \hat{p} = \frac{x}{n} \text{ and } I_T(p) = E\{I_T(Y, p)\} = \frac{np}{p^2} + \frac{n-np}{(1-p)^2}$$

$$= \frac{n}{p} + \frac{n(1-p)}{(1-p)^2} = \frac{n}{p} + \frac{n}{(1-p)}$$

$$= n \frac{1-p+p}{p(1-p)} = \frac{n}{p(1-p)}$$

The test statistics are

$$T_w = (\hat{p} - p_0) \left\{ \frac{n}{\hat{p}(1-\hat{p})} \right\} (\hat{p} - p_0) = \frac{n(\hat{p} - p_0)}{\hat{p}(1-\hat{p})}$$

$$T_s = \left\{ \frac{X - np_0}{p_0(1-p_0)} \right\} \left\{ \frac{n}{p_0(1-p_0)} \right\}^{-1} \left\{ \frac{X - np_0}{p_0(1-p_0)} \right\}$$

$$= \frac{(X - np_0)}{\cancel{p_0(1-p_0)}} \cdot \frac{\cancel{p_0(1-p_0)}}{n} \cdot \frac{(X - np_0)}{p_0(1-p_0)} \cdot \frac{1}{n} \cdot n$$

$$= \left( \frac{X}{n} - p_0 \right) \left( \frac{X}{n} - p_0 \right) \frac{n}{p_0(1-p_0)} = \frac{n(\hat{p} - p_0)}{p_0(1-p_0)} \quad -2 \{L(\theta_0) - L(\hat{\theta}_{MLE})\}$$

$$T_{LR} = -2 \{L(p_0) - L(\hat{p}_{MLE})\}$$

$$= -2 \{X \log p_0 + (n-X) \log(1-p_0) - X \log \hat{p}_{MLE} - (n-X) \log(1-\hat{p}_{MLE})\}$$

$$= -2 \left\{ X \log \frac{p_0}{\hat{p}_{MLE}} + (n-X) \log \frac{1-p_0}{1-\hat{p}_{MLE}} \right\}$$